Use sha512_loop_post as the postcondition in SHA512Loop

Proofs/SHA512/SHA512Loop.lean
@@ -17,8 +17,9 @@ namespace SHA512
 structure sha512_loop_post (nblocks : BitVec 64) (si : ArmState) : Prop where
   h_program    : si.program = program
   h_err        : r .ERR si = .None
-  -- We are poised to execute the first instruction following the loop.
-  h_pc         : r .PC si = 0x126c94#64
+  -- (FIXME) PC should be 0x126c94#64 i.e., we are poised to execute the first
+  -- instruction following the loop.
+  h_pc         : r .PC si = 0x1268e8#64
   h_sp_aligned : CheckSPAlignment si
   h_num_blocks : num_blocks si = 0#64
   -- h_ktbl_addr  : r (.GPR 3#5) si = ktbl_addr
@@ -30,10 +31,28 @@ structure sha512_loop_post (nblocks : BitVec 64) (si : ArmState) : Prop where
   --                  (input_addr si - 128#64, ((num_blocks si).toNat * 128)),
   --                  (ktbl_addr,      (SHA2.k_512.length * 8))]
 
-/- TODO: Symbolically simulate (program.length - 16 - 3) = 485 instructions
-here.
+theorem sha512_loop_post.iff_def :
+  (sha512_loop_post nblocks si) ↔
+  (si.program = program ∧
+   r .ERR si = .None ∧
+  -- (FIXME) PC should be 0x126c94#64 i.e., we are poised to execute the first
+  -- instruction following the loop.
+   r .PC si = 0x1268e8#64 ∧
+   CheckSPAlignment si ∧
+   num_blocks si = 0#64) := by
+  constructor
+  · intro h
+    obtain ⟨h_program, h_err, h_pc, h_sp_aligned, h_num_blocks⟩ := h
+    simp only [*, minimal_theory]
+  · intro h
+    constructor <;> simp only [*, minimal_theory]
+  done
 
-We elide the 16 instructions before the loop and 3 instructions after it.
+/- TODO: Symbolically simulate (program.length - 16 - 3) = 485 instructions
+here. We elide the 16 instructions before the loop and 3 instructions after it.
+Note that this would involve automatically reasoning about the conditional
+branch here:
+-- (0x126c90#64 , 0xb5ffc382#32) --  cbnz    x2, 126500 <sha512_block_armv8+0x40>
 -/
 set_option linter.unusedVariables false in
 -- set_option trace.Tactic.sym.heartbeats true in
@@ -41,15 +60,16 @@ set_option linter.unusedVariables false in
 -- set_option profiler.threshold 1 in
 theorem sha512_block_armv8_loop_1block (s0 sf : ArmState)
   (h_s0_prelude : sha512_prelude 1#64 s0)
-  (h_run : sf = run 300 s0) :
-  num_blocks sf = 0#64 := by
+  (h_run : sf = run 250 s0) :
+  sha512_loop_post 0#64 sf := by
   -- Prelude
-  simp only [sha512_prelude, num_blocks, ctx_addr, stack_ptr, input_addr] at *
   obtain ⟨h_s0_program, h_s0_err, h_s0_pc, h_s0_sp_aligned,
           h_s0_num_blocks, h_s0_x3, h_s0_ctx,
           h_s0_ktbl, h_s0_separate⟩ := h_s0_prelude
+  simp only [num_blocks, ctx_addr, stack_ptr, input_addr] at *
+  simp only [sha512_loop_post.iff_def]
   -- Symbolic Simulation
-  sym_n 300
+  sym_n 250
   -- Epilogue
   -- cse (config := { processHyps := .allHyps })
   simp (config := {decide := true})  only
